examples/riscv/chacha/chacha_symb_exec_quarterroundScript.sml
@@ -107,4 +107,14 @@ val _ = Portable.pprint Tag.pp_tag (tag symb_analysis_thm);
 
 Theorem chacha_other_line_symb_analysis_thm = symb_analysis_thm
 
+val symb_analysis_thm =
+ bir_symb_analysis_thm
+  bir_chacha_prog_def
+  chacha_quarter_round_init_addr_def [chacha_quarter_round_end_addr_def]
+  bspec_chacha_quarter_round_pre_def chacha_birenvtyl_def;
+
+val _ = Portable.pprint Tag.pp_tag (tag symb_analysis_thm);
+
+Theorem chacha_quarter_round_symb_analysis_thm = symb_analysis_thm
+
 val _ = export_theory ();
